Restructure Basic ChaseBranch/ChaseTree results

ExistentialRules/ChaseSequence/Basic.lean
@@ -139,7 +139,6 @@ namespace ChaseBranch
       simp only [eq] at trg_ex
       simp at trg_ex
 
-  -- TODO: check if this simplifies code where we used cb.triggers_exist before
   theorem origin_trg_is_active (cb : ChaseBranch obs kb) (i : Nat) (node : ChaseNode obs kb.rules) (eq : cb.branch.infinite_list (i + 1) = some node) :
       (node.origin.get (cb.origin_isSome i eq)).fst.val.active (cb.prev_node i (by simp [eq])).fact.val := by
     have trg_ex := cb.triggers_exist i
@@ -154,7 +153,6 @@ namespace ChaseBranch
       simp only [← trg_eq]
       exact trg_active
 
-  -- TODO: check if this simplifies code where we used cb.triggers_exist before
   theorem origin_trg_result_yields_next_node_fact (cb : ChaseBranch obs kb) (i : Nat) (node : ChaseNode obs kb.rules) (eq : cb.branch.infinite_list (i + 1) = some node) :
       node.fact.val = (cb.prev_node i (by simp [eq])).fact.val ∪ (node.origin_result (cb.origin_isSome i eq)).toSet := by
     have trg_ex := cb.triggers_exist i
@@ -169,6 +167,356 @@ namespace ChaseBranch
       simp only [← trg_eq]
       unfold ChaseNode.origin_result
       simp
+
+  theorem stepIsSubsetOfAllFollowing (cb : ChaseBranch obs kb) (i : Nat) (node : ChaseNode obs kb.rules) (eq : cb.branch.infinite_list i = some node) :
+      ∀ j, (cb.branch.infinite_list (i + j)).is_none_or (fun node2 => node.fact.val ⊆ node2.fact.val) := by
+    intro j
+    induction j with
+    | zero => rw [Nat.add_zero, eq]; simp only [Option.is_none_or]; apply Set.subset_refl
+    | succ j ih =>
+      rw [Option.is_none_or_iff]
+      intro node2 eq2
+      let prev_node := (cb.prev_node (i + j) (by rw [Nat.add_assoc]; simp [eq2]))
+      apply Set.subset_trans (b := prev_node.fact.val)
+      . rw [Option.is_none_or_iff] at ih
+        specialize ih prev_node (by apply cb.prev_node_eq)
+        exact ih
+      . rw [cb.origin_trg_result_yields_next_node_fact (i + j) node2 eq2]
+        apply Set.subset_union_of_subset_left
+        apply Set.subset_refl
+
+  theorem stepIsSubsetOfResult (cb : ChaseBranch obs kb) : ∀ n : Nat, (cb.branch.infinite_list n).is_none_or (fun fs => fs.fact ⊆ cb.result) := by
+    intro n
+    unfold Option.is_none_or
+
+    cases eq : cb.branch.infinite_list n with
+    | none => simp
+    | some fs =>
+      simp only
+      unfold ChaseBranch.result
+      intro f h
+      exists n
+      rw [Option.is_some_and_iff]
+      exists fs
+
+  theorem constantsInStepAreFromDatabaseOrRuleSet (cb : ChaseBranch obs kb) (i : Nat) (node : ChaseNode obs kb.rules) (eq : cb.branch.infinite_list i = some node) :
+      node.fact.val.constants ⊆ (kb.db.constants.val ∪ kb.rules.head_constants) := by
+    induction i generalizing node with
+    | zero =>
+      rw [cb.database_first] at eq
+      injection eq with eq
+      rw [← eq]
+      rw [Database.toFactSet_constants_same]
+      apply Set.subset_union_of_subset_left
+      apply Set.subset_refl
+    | succ i ih =>
+      let prev_node := (cb.prev_node i (by simp [eq]))
+
+      rw [cb.origin_trg_result_yields_next_node_fact i node eq]
+      unfold FactSet.constants
+      intro c c_mem
+      rcases c_mem with ⟨f, f_mem, c_mem⟩
+      cases f_mem with
+      | inl f_mem =>
+        apply ih prev_node
+        . apply cb.prev_node_eq
+        . exists f
+      | inr f_mem =>
+        unfold ChaseNode.origin_result at f_mem
+        let origin := node.origin.get (cb.origin_isSome i eq)
+        have c_mem : c ∈ FactSet.constants (origin.fst.val.mapped_head[origin.snd.val]).toSet := by unfold FactSet.constants; exists f
+        apply Set.subset_trans (origin.fst.val.mapped_head_constants_subset origin.snd)
+        . intro c c_mem
+          rw [List.mem_toSet, List.mem_append] at c_mem
+          cases c_mem with
+          | inl c_mem =>
+            apply ih prev_node
+            . apply cb.prev_node_eq
+            . rw [List.mem_flatMap] at c_mem
+              rcases c_mem with ⟨t, t_mem, c_mem⟩
+              rw [List.mem_map] at t_mem
+              rcases t_mem with ⟨v, v_mem, t_mem⟩
+              rcases origin.fst.val.rule.frontier_occurs_in_body v v_mem with ⟨a, a_mem, v_mem'⟩
+              exists origin.fst.val.subs.apply_function_free_atom a
+              constructor
+              . have := cb.origin_trg_is_active i node eq
+                apply this.left
+                rw [List.mem_toSet]
+                unfold PreTrigger.mapped_body
+                unfold GroundSubstitution.apply_function_free_conj
+                apply List.mem_map_of_mem
+                exact a_mem
+              . unfold Fact.constants
+                rw [List.mem_flatMap]
+                exists t
+                constructor
+                . unfold GroundSubstitution.apply_function_free_atom
+                  rw [List.mem_map]
+                  exists VarOrConst.var v
+                  constructor
+                  . exact v_mem'
+                  . unfold PreTrigger.subs_for_mapped_head at t_mem
+                    rw [PreTrigger.apply_to_var_or_const_frontier_var] at t_mem
+                    . exact t_mem
+                    . exact v_mem
+                . exact c_mem
+          | inr c_mem =>
+            apply Or.inr
+            exists origin.fst.val.rule
+            constructor
+            . exact origin.fst.property
+            . unfold Rule.head_constants
+              rw [List.mem_flatMap]
+              exists origin.fst.val.rule.head[origin.snd.val]'(by rw [← PreTrigger.length_mapped_head]; exact origin.snd.isLt)
+              constructor
+              . apply List.get_mem
+              . exact c_mem
+        . exact c_mem
+
+  theorem trg_loaded_at_some_step_of_trg_loaded_for_result (cb : ChaseBranch obs kb) : ∀ trg : Trigger obs, trg.loaded cb.result -> ∃ n : Nat, (cb.branch.infinite_list n).is_some_and (fun fs => trg.loaded fs.fact.val) := by
+    intro trg
+    unfold ChaseBranch.result
+    unfold PreTrigger.loaded
+
+    induction trg.mapped_body
+    case nil =>
+      intro _
+      exists 0
+      rw [cb.database_first]
+      simp [Option.is_some_and]
+      intro _ contra
+      simp [List.mem_toSet] at contra
+    case cons hd tl ih =>
+      intro loaded
+      rcases loaded hd (by simp [List.mem_toSet]) with ⟨hd_idx, hd_mem⟩
+      rw [Option.is_some_and_iff] at hd_mem
+
+      rcases ih (by intro e e_mem; rw [List.mem_toSet] at e_mem; apply loaded; simp [List.mem_toSet, e_mem]) with ⟨tl_idx, tl_mem⟩
+      rw [Option.is_some_and_iff] at tl_mem
+
+      exists max hd_idx tl_idx
+      rw [Option.is_some_and_iff]
+
+      cases Decidable.em (tl_idx ≤ hd_idx) with
+      | inl le =>
+        rcases hd_mem with ⟨node, node_eq, hd_mem⟩
+        exists node
+        constructor
+        . rw [Nat.max_eq_left le]
+          exact node_eq
+        . intro e e_mem
+          rw [List.mem_toSet, List.mem_cons] at e_mem
+          cases e_mem with
+          | inl e_mem => rw [e_mem]; exact hd_mem
+          | inr e_mem =>
+            rcases tl_mem with ⟨tl_node, tl_node_eq, tl_mem⟩
+            have := cb.stepIsSubsetOfAllFollowing tl_idx tl_node tl_node_eq (hd_idx - tl_idx)
+            rw [Nat.add_sub_cancel' le] at this
+            rw [node_eq, Option.is_none_or] at this
+            apply this
+            apply tl_mem
+            rw [List.mem_toSet]
+            exact e_mem
+      | inr le =>
+        have le := Nat.le_of_not_le le
+        rcases tl_mem with ⟨node, node_eq, tl_mem⟩
+        exists node
+        constructor
+        . rw [Nat.max_eq_right le]
+          exact node_eq
+        . intro e e_mem
+          rw [List.mem_toSet, List.mem_cons] at e_mem
+          cases e_mem with
+          | inr e_mem => apply tl_mem; rw [List.mem_toSet]; exact e_mem
+          | inl e_mem =>
+            rcases hd_mem with ⟨hd_node, hd_node_eq, hd_mem⟩
+            have := cb.stepIsSubsetOfAllFollowing hd_idx hd_node hd_node_eq (tl_idx - hd_idx)
+            rw [Nat.add_sub_cancel' le] at this
+            rw [node_eq, Option.is_none_or] at this
+            apply this
+            rw [e_mem]
+            exact hd_mem
+
+  theorem trg_active_at_some_step_of_trg_active_for_result (cb : ChaseBranch obs kb) : ∀ trg : Trigger obs, trg.active cb.result -> ∃ n : Nat, (cb.branch.infinite_list n).is_some_and (fun fs => trg.active fs.fact) := by
+    intro trg
+    intro active
+    rcases cb.trg_loaded_at_some_step_of_trg_loaded_for_result trg active.left with ⟨step, loaded_step⟩
+    rw [Option.is_some_and_iff] at loaded_step
+    rcases loaded_step with ⟨node, node_eq, loaded_step⟩
+    exists step
+    rw [Option.is_some_and_iff]
+    exists node
+    constructor
+    . exact node_eq
+    . constructor
+      . exact loaded_step
+      . intro contra
+        apply active.right
+        apply obs.monotone
+        . have := cb.stepIsSubsetOfResult step
+          rw [node_eq, Option.is_none_or] at this
+          exact this
+        . exact contra
+
+  theorem result_models_kb (cb : ChaseBranch obs kb) : cb.result.modelsKb kb := by
+    constructor
+    . unfold FactSet.modelsDb
+      unfold ChaseBranch.result
+      intro f h
+      exists 0
+      rw [cb.database_first, Option.is_some_and]
+      exact h
+    . unfold FactSet.modelsRules
+      intro r h
+      unfold FactSet.modelsRule
+      intro subs subs_loaded
+      apply Classical.byContradiction
+      intro subs_not_obsolete
+      let trg : Trigger obs := ⟨r, subs⟩
+      have trg_loaded : trg.loaded cb.result := by apply subs_loaded
+      have trg_not_obsolete : ¬ obs.cond trg cb.result := by
+        intro contra
+        have obs_impl_sat := obs.cond_implies_trg_is_satisfied contra
+        apply subs_not_obsolete
+        rcases obs_impl_sat with ⟨i, s', obs_impl_sat⟩
+        exists i
+        exists s'
+
+      rcases cb.trg_active_at_some_step_of_trg_active_for_result trg ⟨trg_loaded, trg_not_obsolete⟩ with ⟨step, step_active⟩
+      rw [Option.is_some_and_iff] at step_active
+      rcases step_active with ⟨node, node_eq, step_active⟩
+
+      rcases cb.fairness ⟨trg, by apply h⟩ with ⟨step', step'_not_active⟩
+      rw [Option.is_some_and_iff] at step'_not_active
+      rcases step'_not_active.left with ⟨node', node'_eq, step'_not_active_left⟩
+
+      apply step'_not_active_left
+      constructor
+      . cases Decidable.em (step ≤ step') with
+        | inl le =>
+          apply Set.subset_trans (b := node.fact.val)
+          . exact step_active.left
+          . have := cb.stepIsSubsetOfAllFollowing step node node_eq (step' - step)
+            rw [Nat.add_sub_cancel' le, node'_eq, Option.is_none_or] at this
+            exact this
+        | inr le =>
+          have gt := Nat.gt_of_not_le le
+          apply False.elim
+          have := step'_not_active.right step gt
+          rw [node_eq, Option.is_none_or] at this
+          apply this
+          exact step_active
+      . intro contra
+        apply trg_not_obsolete
+        apply obs.monotone
+        . have := cb.stepIsSubsetOfResult step'
+          rw [node'_eq, Option.is_none_or] at this
+          exact this
+        . exact contra
+
+  theorem funcTermForExisVarInChaseMeansTriggerIsUsed (cb : ChaseBranch obs kb) (i : Nat) {node : ChaseNode obs kb.rules} (eq : cb.branch.infinite_list i = some node)
+      (trg : RTrigger obs kb.rules) (trg_idx : Fin trg.val.mapped_head.length) {v : sig.V} (v_front : ¬ v ∈ trg.val.rule.frontier)
+      (term_in_node : ∃ (f : Fact sig), f ∈ node.fact ∧ (trg.val.functional_term_for_var trg_idx.val v) ∈ f.terms) :
+      ∃ drop_number : Fin i, (cb.branch.infinite_list (i - drop_number.val)).is_some_and (fun prev_node => prev_node.origin.is_some_and (fun origin => trg.equiv origin.fst ∧ trg_idx.val = origin.snd.val)) := by
+    induction i generalizing node with
+    | zero =>
+      rw [cb.database_first] at eq
+      rw [Option.some.injEq] at eq
+      have func_free := kb.db.toFactSet.property.right
+      unfold FactSet.isFunctionFree at func_free
+      rcases term_in_node with ⟨f, f_mem, term_in_node⟩
+      rw [← eq] at f_mem
+      specialize func_free f f_mem
+      unfold Fact.isFunctionFree at func_free
+      specialize func_free _ term_in_node
+      rcases func_free with ⟨_, func_free⟩
+      simp [PreTrigger.functional_term_for_var, GroundTerm.func, GroundTerm.const] at func_free
+    | succ i ih =>
+      let prev_node := (cb.prev_node i (by simp [eq]))
+      cases Classical.em (∃ (f : Fact sig), f ∈ prev_node.fact ∧ (trg.val.functional_term_for_var trg_idx.val v) ∈ f.terms) with
+      | inl term_in_prev_node =>
+        rcases ih (by apply cb.prev_node_eq) term_in_prev_node with ⟨drop, ih⟩
+        exists ⟨drop.val + 1, by simp⟩
+        rw [Nat.add_sub_add_right]
+        exact ih
+      | inr term_not_in_prev_node =>
+        exists ⟨0, by simp⟩
+        rw [Nat.sub_zero, eq]
+        rw [Option.is_some_and]
+        rw [Option.is_some_and_iff]
+
+        let origin := node.origin.get (cb.origin_isSome i eq)
+        exists origin
+        constructor
+        . simp [origin]
+        . rcases term_in_node with ⟨f, f_mem, t_mem⟩
+          rw [cb.origin_trg_result_yields_next_node_fact _ _ eq] at f_mem
+          cases f_mem with
+          | inl f_mem => apply False.elim; apply term_not_in_prev_node; exists f
+          | inr f_mem =>
+            rw [List.mem_toSet] at f_mem
+            unfold ChaseNode.origin_result at f_mem
+            rw [← PreTrigger.apply_subs_for_mapped_head_eq] at f_mem
+            unfold GroundSubstitution.apply_function_free_conj at f_mem
+            rw [List.mem_map] at f_mem
+            rcases f_mem with ⟨a, a_mem, f_mem⟩
+            rw [← f_mem] at t_mem
+            unfold GroundSubstitution.apply_function_free_atom at t_mem
+            rw [List.mem_map] at t_mem
+            rcases t_mem with ⟨voc, voc_mem, t_mem⟩
+            cases voc with
+            | const c => simp [GroundSubstitution.apply_var_or_const, PreTrigger.functional_term_for_var, GroundTerm.func, GroundTerm.const] at t_mem
+            | var v2 =>
+              have v2_front : ¬ v2 ∈ origin.fst.val.rule.frontier := by
+                intro contra
+                rw [PreTrigger.apply_subs_for_var_or_const_eq, PreTrigger.apply_to_var_or_const_frontier_var _ _ _ contra] at t_mem
+                apply term_not_in_prev_node
+                rcases origin.fst.val.rule.frontier_occurs_in_body _ contra with ⟨b, b_mem, v2_mem⟩
+                exists origin.fst.val.subs.apply_function_free_atom b
+                constructor
+                . have active := cb.origin_trg_is_active i node eq
+                  apply active.left
+                  rw [List.mem_toSet]
+                  unfold PreTrigger.mapped_body
+                  unfold GroundSubstitution.apply_function_free_conj
+                  apply List.mem_map_of_mem
+                  exact b_mem
+                . rw [← t_mem]
+                  unfold GroundSubstitution.apply_function_free_atom
+                  rw [List.mem_map]
+                  exists VarOrConst.var v2
+              rw [PreTrigger.apply_subs_for_var_or_const_eq, PreTrigger.apply_to_var_or_const_non_frontier_var _ _ _ v2_front] at t_mem
+
+              have := RTrigger.funcTermForExisVarInMultipleTriggersMeansTheyAreTheSame
+                trg
+                origin.fst
+                ⟨trg_idx.val, by rw [← PreTrigger.length_mapped_head]; exact trg_idx.isLt⟩
+                ⟨origin.snd.val, by rw [← PreTrigger.length_mapped_head]; exact origin.snd.isLt⟩
+                v
+                v2
+                v_front
+                v2_front
+              apply this
+              rw [PreTrigger.apply_to_var_or_const_non_frontier_var _ _ _ v_front]
+              rw [PreTrigger.apply_to_var_or_const_non_frontier_var _ _ _ v2_front]
+              exact Eq.symm t_mem
+
+  theorem funcTermForExisVarInChaseMeansTriggerResultOccurs (cb : ChaseBranch obs kb) (i : Nat) {node : ChaseNode obs kb.rules} (eq : cb.branch.infinite_list i = some node)
+      (trg : RTrigger obs kb.rules) (trg_idx : Fin trg.val.mapped_head.length) {v : sig.V} (v_front : ¬ v ∈ trg.val.rule.frontier)
+      (term_in_node : ∃ (f : Fact sig), f ∈ node.fact ∧ (trg.val.functional_term_for_var trg_idx.val v) ∈ f.terms) :
+      trg.val.mapped_head[trg_idx.val].toSet ⊆ node.fact.val := by
+    rcases cb.funcTermForExisVarInChaseMeansTriggerIsUsed i eq trg trg_idx v_front term_in_node with ⟨drop, h⟩
+    rw [Option.is_some_and_iff] at h
+    rcases h with ⟨prev_node, prev_node_eq, h⟩
+    rw [Option.is_some_and_iff] at h
+    rcases h with ⟨origin, origin_eq, h⟩
+    simp only [PreTrigger.result_eq_of_equiv _ _ h.left, h.right]
+    have := prev_node.fact_contains_origin_result
+    rw [origin_eq, Option.is_none_or] at this
+    apply Set.subset_trans this
+    have := cb.stepIsSubsetOfAllFollowing (i - drop.val) prev_node prev_node_eq drop.val
+    rw [Nat.sub_add_cancel (Nat.le_of_lt drop.isLt), eq, Option.is_none_or] at this
+    exact this
 
 end ChaseBranch
 
@@ -192,6 +540,7 @@ structure ChaseTree (obs : ObsoletenessCondition sig) (kb : KnowledgeBase sig) w
     (tree.get node).is_none_or (fun fs => ¬ trg.val.active fs.fact)
 
 namespace ChaseTree
+
   variable {obs : ObsoletenessCondition sig} {kb : KnowledgeBase sig}
 
   def branches (ct : ChaseTree obs kb) : Set (ChaseBranch obs kb) := fun branch =>
@@ -201,689 +550,259 @@ namespace ChaseTree
     branch.branch ∈ ct.tree.branches_through node
 
   def result (ct : ChaseTree obs kb) : Set (FactSet sig) := fun fs => ∃ branch, branch ∈ ct.branches ∧ branch.result = fs
-end ChaseTree
 
-
-variable {obs : ObsoletenessCondition sig} {kb : KnowledgeBase sig}
-
-theorem chaseBranchSetIsSubsetOfNext (cb : ChaseBranch obs kb) : ∀ n : Nat,
-  match cb.branch.infinite_list n with
-  | .none => cb.branch.infinite_list (n+1) = none
-  | .some fs => (cb.branch.infinite_list (n+1)).is_none_or (fun fs2 => fs.fact.val ⊆ fs2.fact.val) :=
-by
-  intro n
-  cases eq : cb.branch.infinite_list n with
-  | none =>
-    simp
-    have dec : Decidable (cb.branch.infinite_list (n+1) = none) := Option.decidable_eq_none
-    apply dec.byContradiction
-    intro contra
-    let n' : Fin (n+1) := ⟨n, by simp⟩
-    have : ¬ cb.branch.infinite_list n' = none := by apply cb.branch.no_holes; apply contra
-    contradiction
-  | some fs =>
-    simp
-    cases eq2 : cb.branch.infinite_list (n+1) with
-    | none => simp [Option.is_none_or]
-    | some fs2 =>
-      simp [Option.is_none_or]
-      intro f h
-      have trg_ex_n := cb.triggers_exist n
-      simp [eq, Option.is_none_or] at trg_ex_n
-      cases trg_ex_n with
-      | inl g =>
-        cases g with | intro trg h_trg =>
-          cases h_trg.right with | intro i h_i =>
-            rw [eq2] at h_i
-            injection h_i with h_i
-            rw [← h_i]
-            simp [Set.element, Set.union]
-            apply Or.inl
-            exact h
-      | inr g =>
-        have g_right := g.right
-        rw [eq2] at g_right
-        contradiction
-
-theorem chaseTreeSetIsSubsetOfEachNext (ct : ChaseTree obs kb) : ∀ address : List Nat,
-  match ct.tree.get address with
-  | .none => ct.tree.children address = []
-  | .some fs => ∀ fs2, fs2 ∈ ct.tree.children address -> fs.fact.val ⊆ fs2.fact.val :=
-by
-  intro address
-  cases eq : ct.tree.get address with
-  | none => simp; apply FiniteDegreeTree.children_empty_of_get_eq_none; exact eq
-  | some fs =>
-    simp
-    intro fs2 h
-    have trg_ex_addr := ct.triggers_exist address
-    simp [eq, Option.is_none_or] at trg_ex_addr
-    cases trg_ex_addr with
-    | inl g =>
-      cases g with | intro trg h_trg =>
-        rw [← h_trg.right] at h
-        rw [List.mem_map] at h
-        cases h with | intro head h_head =>
-          rw [← h_head.right]
-          intro f h
-          apply Or.inl
-          exact h
-    | inr g =>
-      rw [g.right] at h
-      contradiction
-
-theorem chaseBranchSetIsSubsetOfAllFollowing (cb : ChaseBranch obs kb) : ∀ (n m : Nat),
-  match cb.branch.infinite_list n with
-  | .none => cb.branch.infinite_list (n+m) = none
-  | .some fs => (cb.branch.infinite_list (n+m)).is_none_or (fun fs2 => fs.fact.val ⊆ fs2.fact.val) :=
-by
-  intro n m
-  induction m with
-  | zero =>
-    cases eq : cb.branch.infinite_list n with
-    | none => simp; exact eq
-    | some fs => simp [Option.is_none_or, eq, Set.subset]
-  | succ m ih =>
-    cases eq : cb.branch.infinite_list n with
-    | none =>
-      simp
-      simp [eq] at ih
-      have step := chaseBranchSetIsSubsetOfNext cb (n+m)
-      simp [ih] at step
-      exact step
-    | some fs =>
-      simp
-      simp [eq, Option.is_none_or] at ih
-      have step := chaseBranchSetIsSubsetOfNext cb (n+m)
-      cases eq2 : cb.branch.infinite_list (n+m) with
-      | none => simp [eq2] at step; rw [← Nat.add_assoc, step, Option.is_none_or]; simp
-      | some fs2 =>
-        simp [eq2] at step; simp [eq2] at ih; rw [← Nat.add_assoc]
-        cases eq3 : cb.branch.infinite_list (n+m+1) with
-        | none => simp [Option.is_none_or]
-        | some fs3 =>
-          simp [Option.is_none_or]; simp [eq3, Option.is_none_or] at step;
-          apply Set.subset_trans; exact ih; exact step
-
-theorem chaseTreeSetIsSubsetOfAllFollowing (ct : ChaseTree obs kb) : ∀ (n m : List Nat),
-  match ct.tree.get n with
-  | .none => ct.tree.get (m ++ n) = none
-  | .some fs => (ct.tree.get (m ++ n)).is_none_or (fun fs2 => fs.fact.val ⊆ fs2.fact.val) :=
-by
-  intro n m
-  induction m with
-  | nil =>
-    cases eq : ct.tree.get n with
-    | none => simp; exact eq
-    | some fs => simp [Option.is_none_or, eq, Set.subset]
-  | cons i m ih =>
-    cases eq : ct.tree.get n with
-    | none =>
-      simp
-      simp [eq] at ih
-      have step := chaseTreeSetIsSubsetOfEachNext ct (m ++ n)
-      simp [ih] at step
-      apply FiniteDegreeTree.each_successor_none_of_children_empty
-      apply step
-    | some fs =>
-      simp
-      simp [eq, Option.is_none_or] at ih
-      have step := chaseTreeSetIsSubsetOfEachNext ct (m ++ n)
-      cases eq2 : ct.tree.get (m ++ n) with
-      | none =>
-        simp [eq2] at step
-        unfold Option.is_none_or
-        have helper := ct.tree.each_successor_none_of_children_empty (m ++ n) step
-        rw [helper]
-        simp
-      | some fs2 =>
-        simp [eq2] at step; simp [eq2] at ih
-        cases eq3 : ct.tree.get (i :: (m ++ n)) with
-        | none => simp [Option.is_none_or]
-        | some fs3 =>
-          simp [Option.is_none_or]
-          apply Set.subset_trans
-          . exact ih
-          . apply step
-            rw [ct.tree.in_children_iff_index_exists]
-            exists i
-
-theorem chaseBranchSetIsSubsetOfResult (cb : ChaseBranch obs kb) : ∀ n : Nat, (cb.branch.infinite_list n).is_none_or (fun fs => fs.fact ⊆ cb.result) := by
-  intro n
-  unfold Option.is_none_or
-
-  cases eq : cb.branch.infinite_list n with
-  | none => simp
-  | some fs =>
-    simp
-    unfold ChaseBranch.result
-    intro f h
-    simp [Set.element]
-    exists n
-    unfold Option.is_some_and
-    simp [eq]
-    exact h
-
-theorem chaseTreeSetIsSubsetOfResult (ct : ChaseTree obs kb) : ∀ node : List Nat, (ct.tree.get node).is_none_or (fun fs => ∀ branch, branch ∈ ct.branches_through node -> fs.fact ⊆ branch.result) := by
-  intro node
-  unfold Option.is_none_or
-
-  cases eq : ct.tree.get node with
-  | none => simp
-  | some fs =>
-    simp
-    intro branch branch_through_node
-    have : branch.branch.infinite_list node.length = ct.tree.get node := by
-      unfold ChaseTree.branches_through at branch_through_node
-      unfold FiniteDegreeTree.branches_through at branch_through_node
-      unfold PossiblyInfiniteTree.branches_through at branch_through_node
-      unfold InfiniteTreeSkeleton.branches_through at branch_through_node
-      simp [Set.element] at branch_through_node
-      rcases branch_through_node with ⟨nodes, eq, eq2⟩
-      rw [eq node.length, eq2]
-      rfl
-
-    have branch_subs_result := chaseBranchSetIsSubsetOfResult branch node.length
-    rw [this] at branch_subs_result
-    simp [eq, Option.is_none_or] at branch_subs_result
-    apply branch_subs_result
-
-theorem constantsInChaseBranchAreFromDatabase (cb : ChaseBranch obs kb) : ∀ n : Nat, (cb.branch.infinite_list n).is_none_or (fun fs => fs.fact.val.constants ⊆ (kb.db.constants.val ∪ kb.rules.head_constants)) := by
-  intro n
-  induction n with
-  | zero =>
-    rw [cb.database_first, Option.is_none_or]
-    simp only
-    rw [Database.toFactSet_constants_same]
-    apply Set.subset_union_of_subset_left
-    apply Set.subset_refl
-  | succ n ih =>
-    cases eq_node : cb.branch.infinite_list (n+1) with
-    | none => simp [Option.is_none_or]
+  theorem predecessor_isSome_of_isSome (ct : ChaseTree obs kb) (path : List Nat) (i : Nat) (isSome : (ct.tree.get (i::path)).isSome) :
+      (ct.tree.get path).isSome := by
+    cases eq : ct.tree.get (i::path) with
+    | none => rw [eq] at isSome; simp at isSome
     | some node =>
-      cases eq_prev : cb.branch.infinite_list n with
+      cases eq_prev : ct.tree.get path with
+      | some prev => simp
       | none =>
-        have no_holes := cb.branch.no_holes (n+1)
-        simp [eq_node] at no_holes
-        specialize no_holes ⟨n, by simp⟩
-        simp [eq_prev] at no_holes
-      | some prev =>
-        rw [Option.is_none_or]
-        rw [eq_prev, Option.is_none_or] at ih
+        apply False.elim
+        have no_holes := ct.tree.tree.no_orphans (i::path)
+        unfold FiniteDegreeTree.get at eq
+        unfold PossiblyInfiniteTree.get at eq
+        simp [eq] at no_holes
+        specialize no_holes path [i] (by simp)
+        apply no_holes
+        exact eq_prev
 
-        have trg_ex := cb.triggers_exist n
-        rw [eq_prev, Option.is_none_or] at trg_ex
-        cases trg_ex with
-        | inr trg_ex => unfold not_exists_trigger_opt_fs at trg_ex; rw [eq_node] at trg_ex; simp at trg_ex
-        | inl trg_ex =>
-          unfold exists_trigger_opt_fs at trg_ex
-          rcases trg_ex with ⟨trg, trg_active, disj_index, trg_ex⟩
-          rw [eq_node] at trg_ex
-          injection trg_ex with trg_ex
-          rw [← trg_ex]
-          simp only
-          unfold FactSet.constants
-          intro c c_mem
-          rcases c_mem with ⟨f, f_mem, c_mem⟩
-          cases f_mem with
-          | inl f_mem =>
-            apply ih
-            exists f
-          | inr f_mem =>
-            unfold Fact.constants at c_mem
-            rw [List.mem_toSet] at f_mem
-            unfold PreTrigger.mapped_head at f_mem
-            simp at f_mem
-            rcases f_mem with ⟨a, a_mem, f_eq⟩
-            unfold PreTrigger.apply_to_function_free_atom at f_eq
-            rw [← f_eq] at c_mem
-            simp only at c_mem
+  def prev_node (ct : ChaseTree obs kb) (path : List Nat) (i : Nat) (isSome : (ct.tree.get (i::path)).isSome) : ChaseNode obs kb.rules :=
+    (ct.tree.get path).get (ct.predecessor_isSome_of_isSome path i isSome)
 
-            rw [List.mem_flatMap] at c_mem
-            rcases c_mem with ⟨tree, tree_mem, c_mem⟩
-            rw [List.mem_map] at tree_mem
-            rcases tree_mem with ⟨voc, voc_mem, tree_eq⟩
-            unfold PreTrigger.apply_to_var_or_const at tree_eq
+  theorem prev_node_eq (ct : ChaseTree obs kb) (path : List Nat) (i : Nat) (isSome : (ct.tree.get (i::path)).isSome) :
+      ct.tree.get path = some (ct.prev_node path i isSome) := by
+    simp [prev_node]
 
-            cases voc with
-            | const d =>
-              simp only [Function.comp_apply, PreTrigger.skolemize_var_or_const, GroundSubstitution.apply_skolem_term, VarOrConst.skolemize] at tree_eq
-              apply Or.inr
-              unfold RuleSet.head_constants
-              exists trg.val.rule
-              constructor
-              . exact trg.property
-              . unfold Rule.head_constants
-                rw [List.mem_flatMap]
-                exists trg.val.rule.head[disj_index.val]'(by rw [← PreTrigger.length_mapped_head]; exact disj_index.isLt)
-                constructor
-                . simp
-                . unfold FunctionFreeConjunction.consts
-                  rw [List.mem_flatMap]
-                  exists a
-                  constructor
-                  . exact a_mem
-                  . unfold FunctionFreeAtom.constants
-                    apply VarOrConst.mem_filterConsts_of_const
-                    rw [← tree_eq] at c_mem
-                    rw [GroundTerm.constants_const, List.mem_singleton] at c_mem
-                    rw [c_mem]
-                    exact voc_mem
-            | var v =>
-              simp only [Function.comp_apply, PreTrigger.skolemize_var_or_const, GroundSubstitution.apply_skolem_term, VarOrConst.skolemize] at tree_eq
-
-              cases Decidable.em (v ∈ trg.val.rule.frontier) with
-              | inl v_frontier =>
-                simp [v_frontier] at tree_eq
-
-                apply ih
-                rcases (trg.val.rule.frontier_occurs_in_body _ v_frontier) with ⟨b, b_mem, v_mem⟩
-                exists trg.val.subs.apply_function_free_atom b
-                constructor
-                . apply trg_active.left
-                  rw [List.mem_toSet]
-                  unfold PreTrigger.mapped_body
-                  simp only [GroundSubstitution.apply_function_free_conj]
-                  rw [List.mem_map]
-                  exists b
-                . unfold Fact.constants
-                  rw [List.mem_flatMap]
-                  exists tree
-                  constructor
-                  . rw [← tree_eq]
-                    unfold GroundSubstitution.apply_function_free_atom
-                    rw [List.mem_map]
-                    exists (VarOrConst.var v)
-                  . exact c_mem
-              | inr v_frontier =>
-                simp [v_frontier] at tree_eq
-                rw [← tree_eq] at c_mem
-                rw [GroundTerm.constants_func, List.mem_flatMap] at c_mem
-                rcases c_mem with ⟨tree, tree_mem, c_mem⟩
-                rw [List.mem_map] at tree_mem
-                rcases tree_mem with ⟨v, v_frontier, tree_eq⟩
-
-                -- from here its the same as in the inl case
-                apply ih
-                rcases (trg.val.rule.frontier_occurs_in_body _ v_frontier) with ⟨b, b_mem, v_mem⟩
-                exists trg.val.subs.apply_function_free_atom b
-                constructor
-                . apply trg_active.left
-                  rw [List.mem_toSet]
-                  unfold PreTrigger.mapped_body
-                  simp only [GroundSubstitution.apply_function_free_conj]
-                  rw [List.mem_map]
-                  exists b
-                . unfold Fact.constants
-                  rw [List.mem_flatMap]
-                  exists tree
-                  constructor
-                  . rw [← tree_eq]
-                    unfold GroundSubstitution.apply_function_free_atom
-                    rw [List.mem_map]
-                    exists (VarOrConst.var v)
-                  . exact c_mem
-
-theorem trgLoadedForChaseResultMeansLoadedAtSomeIndex (cb : ChaseBranch obs kb) : ∀ trg : Trigger obs, trg.loaded cb.result -> ∃ n : Nat, (cb.branch.infinite_list n).is_some_and (fun fs => trg.loaded fs.fact) := by
-  intro trg
-  unfold ChaseBranch.result
-  unfold PreTrigger.loaded
-
-  induction trg.mapped_body
-  case nil =>
-    intro _
-    exists 0
-    rw [cb.database_first]
-    simp [Option.is_some_and]
-    intro _ contra
-    contradiction
-  case cons head tail ih =>
-    intro loaded
-    have ex_head_n := loaded head
-    simp [Set.element, List.toSet, Set.union] at ex_head_n
-
-    have ex_tail_n := by
-      apply ih
-      simp [List.toSet] at loaded
-      have ⟨ _, tailSubs ⟩ := (Set.union_subset_iff_both_subset _ _ _).mp loaded
-      exact tailSubs
-    cases ex_head_n with | intro i hi =>
-      cases ex_tail_n with | intro j hj =>
-        exists Nat.max i j
-        simp [List.toSet]
-
-        have max_help_left : ∀ a b : Nat, a ≤ Nat.max a b := by
-          intro a b
-          simp [Nat.max_def]
-          cases Decidable.em (a ≤ b)
-          case inl h => simp [h]
-          case inr h => simp [h]
-        have max_help_right : ∀ a b : Nat, b ≤ Nat.max a b := by
-          intro a b
-          simp [Nat.max_def]
-          split -- seems to be the same as the following above: cases Decidable.em (a ≤ b)
-          case isTrue h => simp [h]
-          case isFalse h => apply Nat.le_of_lt; apply Nat.lt_of_succ_le; rw [← Nat.not_le_eq]; exact h
-        have help_i : i ≤ Nat.max i j := by apply max_help_left
-        have help_j : j ≤ Nat.max i j := by apply max_help_right
-
-        unfold Option.is_some_and
-        split
-        case h_1 heq =>
-          simp [Nat.max_def] at heq
-          split at heq
-          . rw [heq] at hj
-            simp [Option.is_some_and] at hj
-          . rw [heq] at hi
-            simp [Option.is_some_and] at hi
-
-        case h_2 heq =>
-          simp
-          rw [Set.union_subset_iff_both_subset]
-          constructor
-          . unfold Option.is_some_and at hi
-            split at hi
-            . contradiction
-            case h_2 a heq2 =>
-              apply Set.subset_trans (b := a.fact)
-              . intro e he
-                simp [Set.element] at he
-                rw [he]
-                assumption
-              . cases Nat.le.dest help_i with | intro m hm =>
-                have subsOfAllFollowing := chaseBranchSetIsSubsetOfAllFollowing cb i m
-                rw [heq2] at subsOfAllFollowing
-                simp at subsOfAllFollowing
-                rw [← hm] at heq
-                rw [heq] at subsOfAllFollowing
-                simp [Option.is_none_or] at subsOfAllFollowing
-                exact subsOfAllFollowing
-          . cases Nat.le.dest help_j with | intro m hm =>
-              have subsOfAllFollowing := chaseBranchSetIsSubsetOfAllFollowing cb j m
-              split at subsOfAllFollowing
-              . rw [hm, heq] at subsOfAllFollowing; contradiction
-              case h_2 heq2 =>
-                rw [heq2] at hj
-                simp [Option.is_some_and] at hj
-                rw [← hm] at heq
-                rw [heq] at subsOfAllFollowing
-                simp [Option.is_none_or] at subsOfAllFollowing
-                apply Set.subset_trans
-                . exact hj
-                . exact subsOfAllFollowing
-
-theorem trgActiveForChaseResultMeansActiveAtSomeIndex (cb : ChaseBranch obs kb) : ∀ trg : Trigger obs, trg.active cb.result -> ∃ n : Nat, (cb.branch.infinite_list n).is_some_and (fun fs => trg.active fs.fact) := by
-  intro trg
-  unfold Trigger.active
-  simp
-  intro loaded active
-  have trgLoadedForN := trgLoadedForChaseResultMeansLoadedAtSomeIndex cb trg loaded
-  cases trgLoadedForN with | intro n loadedN =>
-    exists n
-    unfold Option.is_some_and
-    split
-    case h_1 heq => rw [heq] at loadedN; simp [Option.is_some_and] at loadedN
-    case h_2 heq =>
+  theorem origin_isSome (ct : ChaseTree obs kb) (path : List Nat) (i : Nat) {node : ChaseNode obs kb.rules}
+      (eq : ct.tree.get (i::path) = some node) : node.origin.isSome := by
+    have trg_ex := ct.triggers_exist path
+    rw [prev_node_eq _ _ i (by simp [eq]), Option.is_none_or] at trg_ex
+    cases trg_ex with
+    | inl trg_ex =>
+      unfold exists_trigger_list at trg_ex
+      unfold exists_trigger_list_condition at trg_ex
+      rcases trg_ex with ⟨trg, _, trg_eq⟩
+      let i_fin : Fin (ct.tree.children path).length := ⟨i, by
+        unfold FiniteDegreeTree.get at eq
+        rw [← ct.tree.tree.getElem_children_eq_get path i] at eq
+        rw [← ct.tree.getElem_children_eq_getElem_lifted_children path] at eq
+        rw [List.getElem?_eq_some_iff] at eq
+        rcases eq with ⟨h, _⟩
+        exact h
+      ⟩
+      have := List.getElem_of_eq (Eq.symm trg_eq) i_fin.isLt
+      rw [List.getElem_map] at this
+      simp only at this
+      rw [← Option.some.injEq] at this
+      rw [ct.tree.getElem_children_eq_get path i_fin] at this
+      simp only [i_fin, eq] at this
+      rw [Option.some.injEq] at this
+      rw [this]
       simp
-      constructor
-      . rw [heq] at loadedN; simp [Option.is_some_and] at loadedN; exact loadedN
-      . intro contra
-        apply active
-        apply obs.monotone
-        . have subsetOfResult := chaseBranchSetIsSubsetOfResult cb n
-          rw [heq] at subsetOfResult
-          simp [Option.is_none_or] at subsetOfResult
-          apply subsetOfResult
-        . apply contra
+    | inr trg_ex =>
+      unfold not_exists_trigger_list at trg_ex
+      have := ct.tree.each_successor_none_of_children_empty _ trg_ex.right i
+      rw [this] at eq
+      simp at eq
 
-theorem funcTermForExisVarInChaseTreeMeansTriggerIsUsed (ct : ChaseTree obs kb) (trg : RTrigger obs kb.rules) (result_index : Fin trg.val.mapped_head.length) (var : sig.V) (node : ChaseNode obs kb.rules) (node_path : List Nat) : some node = ct.tree.get node_path ∧ (¬ var ∈ trg.val.rule.frontier) ∧ (∃ f: Fact sig, f ∈ node.fact ∧ (trg.val.apply_to_var_or_const result_index (VarOrConst.var var)) ∈ f.terms) -> ∃ drop_number : Fin node_path.length, (ct.tree.get (node_path.drop drop_number.val)).is_some_and (fun prev_node => prev_node.origin.is_some_and (fun origin => trg.equiv origin.fst ∧ result_index.val = origin.snd.val)) := by
-  intro ⟨node_is_at_path, var_not_in_frontier, exis_f⟩
-  induction node_path generalizing node with
-  | nil =>
-    cases exis_f with | intro f hf =>
-      let ⟨f_in_db, functional_term_in_f⟩ := hf
-      rw [ct.database_first] at node_is_at_path
-      injection node_is_at_path with node_is_at_path
-      rw [node_is_at_path] at f_in_db
-      simp only at f_in_db
-      have isFunctionFree := kb.db.toFactSet.property.right
-      specialize isFunctionFree _ f_in_db
-      specialize isFunctionFree (trg.val.apply_to_var_or_const (result_index.val) (VarOrConst.var var)) functional_term_in_f
-      rcases isFunctionFree with ⟨c, isFunctionFree⟩
-      simp [PreTrigger.apply_to_var_or_const, PreTrigger.skolemize_var_or_const, GroundSubstitution.apply_skolem_term, VarOrConst.skolemize, var_not_in_frontier, GroundTerm.const, GroundTerm.func] at isFunctionFree
-  | cons head tail ih =>
-    cases eq : ct.tree.get tail with
-    | none =>
-      apply False.elim
-      apply ct.tree.tree.no_orphans (head::tail) _ ⟨tail, by exists [head]⟩
-      unfold FiniteDegreeTree.get at eq
-      unfold PossiblyInfiniteTree.get at eq
-      exact eq
-      unfold FiniteDegreeTree.get at node_is_at_path
-      unfold PossiblyInfiniteTree.get at node_is_at_path
-      rw [← node_is_at_path]
-      simp
-    | some tail_node =>
-      -- TODO: this should actually be decidable but we need to change the implementation for this
-      cases Classical.em (∃ f: Fact sig, f ∈ tail_node.fact ∧ (trg.val.subs.apply_skolem_term (VarOrConst.skolemize trg.val.rule.id result_index.val trg.val.rule.frontier (VarOrConst.var var))) ∈ f.terms) with
-      | inl f_in_j =>
-        cases ih tail_node (Eq.symm eq) f_in_j with | intro k _ =>
-          exists ⟨k+1, by simp⟩
-      | inr f_not_in_j =>
+  theorem origin_trg_is_active (ct : ChaseTree obs kb) (path : List Nat) (i : Nat) (node : ChaseNode obs kb.rules) (eq : ct.tree.get (i::path) = some node) :
+      (node.origin.get (ct.origin_isSome path i eq)).fst.val.active (ct.prev_node path i (by simp [eq])).fact.val := by
+    have trg_ex := ct.triggers_exist path
+    rw [prev_node_eq _ _ i (by simp [eq]), Option.is_none_or] at trg_ex
+    cases trg_ex with
+    | inl trg_ex =>
+      unfold exists_trigger_list at trg_ex
+      unfold exists_trigger_list_condition at trg_ex
+      rcases trg_ex with ⟨trg, trg_active, trg_eq⟩
+      let i_fin : Fin (ct.tree.children path).length := ⟨i, by
+        unfold FiniteDegreeTree.get at eq
+        rw [← ct.tree.tree.getElem_children_eq_get path i] at eq
+        rw [← ct.tree.getElem_children_eq_getElem_lifted_children path] at eq
+        rw [List.getElem?_eq_some_iff] at eq
+        rcases eq with ⟨h, _⟩
+        exact h
+      ⟩
+      have := List.getElem_of_eq (Eq.symm trg_eq) i_fin.isLt
+      rw [List.getElem_map] at this
+      simp only at this
+      rw [← Option.some.injEq] at this
+      rw [ct.tree.getElem_children_eq_get path i_fin] at this
+      simp only [i_fin, eq] at this
+      rw [Option.some.injEq] at this
+      simp [this, trg_active]
+    | inr trg_ex =>
+      unfold not_exists_trigger_list at trg_ex
+      have := ct.tree.each_successor_none_of_children_empty _ trg_ex.right i
+      rw [this] at eq
+      simp at eq
+
+  theorem origin_trg_result_yields_next_node_fact (ct : ChaseTree obs kb) (path : List Nat) (i : Nat) (node : ChaseNode obs kb.rules) (eq : ct.tree.get (i::path) = some node) :
+      node.fact.val = (ct.prev_node path i (by simp [eq])).fact.val ∪ (node.origin_result (ct.origin_isSome path i eq)).toSet := by
+    have trg_ex := ct.triggers_exist path
+    rw [prev_node_eq _ _ i (by simp [eq]), Option.is_none_or] at trg_ex
+    cases trg_ex with
+    | inl trg_ex =>
+      unfold exists_trigger_list at trg_ex
+      unfold exists_trigger_list_condition at trg_ex
+      rcases trg_ex with ⟨trg, trg_active, trg_eq⟩
+      let i_fin : Fin (ct.tree.children path).length := ⟨i, by
+        unfold FiniteDegreeTree.get at eq
+        rw [← ct.tree.tree.getElem_children_eq_get path i] at eq
+        rw [← ct.tree.getElem_children_eq_getElem_lifted_children path] at eq
+        rw [List.getElem?_eq_some_iff] at eq
+        rcases eq with ⟨h, _⟩
+        exact h
+      ⟩
+      have := List.getElem_of_eq (Eq.symm trg_eq) i_fin.isLt
+      rw [List.getElem_map] at this
+      simp only at this
+      rw [← Option.some.injEq] at this
+      rw [ct.tree.getElem_children_eq_get path i_fin] at this
+      simp only [i_fin, eq] at this
+      rw [Option.some.injEq] at this
+      unfold ChaseNode.origin_result
+      have i_lt : i < trg.val.mapped_head.length := by
+        have : trg.val.mapped_head.length = (ct.tree.children path).length := by
+          rw [← trg_eq]
+          rw [List.length_map, List.length_attach, List.length_enum_with_lt]
+        rw [this]
+        exact i_fin.isLt
+      have origin_eq : node.origin.get (by simp [this]) = ⟨trg, ⟨i, i_lt⟩⟩ := by simp only [this]; simp [List.enum_with_lt_getElem_fst_eq_index i_lt]
+      have idx_eq : (node.origin.get (by simp [this])).snd.val = i := by rw [origin_eq]
+      simp only [this]
+      simp [List.enum_with_lt_getElem_snd_eq_getElem i_lt, idx_eq]
+    | inr trg_ex =>
+      unfold not_exists_trigger_list at trg_ex
+      have := ct.tree.each_successor_none_of_children_empty _ trg_ex.right i
+      rw [this] at eq
+      simp at eq
+
+  theorem stepIsSubsetOfAllFollowing (ct : ChaseTree obs kb) (path : List Nat) (node : ChaseNode obs kb.rules) (eq : ct.tree.get path = some node) :
+      ∀ path2, (ct.tree.get (path2 ++ path)).is_none_or (fun node2 => node.fact.val ⊆ node2.fact.val) := by
+    intro path2
+    induction path2 with
+    | nil => rw [List.nil_append, eq]; simp only [Option.is_none_or]; apply Set.subset_refl
+    | cons hd tl ih =>
+      rw [Option.is_none_or_iff]
+      intro node2 eq2
+      let prev_node := (ct.prev_node (tl ++ path) hd (by rw [← List.cons_append, eq2]; simp))
+      apply Set.subset_trans (b := prev_node.fact.val)
+      . rw [Option.is_none_or_iff] at ih
+        specialize ih prev_node (by apply ct.prev_node_eq)
+        exact ih
+      . rw [ct.origin_trg_result_yields_next_node_fact (tl ++ path) hd node2 eq2]
+        apply Set.subset_union_of_subset_left
+        apply Set.subset_refl
+
+  theorem result_models_kb (ct : ChaseTree obs kb) : ∀ fs, fs ∈ ct.result -> fs.modelsKb kb := by
+    intro fs fs_mem
+    rcases fs_mem with ⟨branch, _, fs_mem⟩
+    rw [← fs_mem]
+    apply branch.result_models_kb
+
+  theorem funcTermForExisVarInChaseMeansTriggerIsUsed (ct : ChaseTree obs kb) (path : List Nat) {node : ChaseNode obs kb.rules} (eq : ct.tree.get path = some node)
+      (trg : RTrigger obs kb.rules) (trg_idx : Fin trg.val.mapped_head.length) {v : sig.V} (v_front : ¬ v ∈ trg.val.rule.frontier)
+      (term_in_node : ∃ (f : Fact sig), f ∈ node.fact ∧ (trg.val.functional_term_for_var trg_idx.val v) ∈ f.terms) :
+      ∃ drop_number : Fin path.length, (ct.tree.get (path.drop drop_number.val)).is_some_and (fun prev_node => prev_node.origin.is_some_and (fun origin => trg.equiv origin.fst ∧ trg_idx.val = origin.snd.val)) := by
+    induction path generalizing node with
+    | nil =>
+      rw [ct.database_first] at eq
+      rw [Option.some.injEq] at eq
+      have func_free := kb.db.toFactSet.property.right
+      unfold FactSet.isFunctionFree at func_free
+      rcases term_in_node with ⟨f, f_mem, term_in_node⟩
+      rw [← eq] at f_mem
+      specialize func_free f f_mem
+      unfold Fact.isFunctionFree at func_free
+      specialize func_free _ term_in_node
+      rcases func_free with ⟨_, func_free⟩
+      simp [PreTrigger.functional_term_for_var, GroundTerm.func, GroundTerm.const] at func_free
+    | cons i path ih =>
+      let prev_node := (ct.prev_node path i (by simp [eq]))
+      cases Classical.em (∃ (f : Fact sig), f ∈ prev_node.fact ∧ (trg.val.functional_term_for_var trg_idx.val v) ∈ f.terms) with
+      | inl term_in_prev_node =>
+        rcases ih (by apply ct.prev_node_eq) term_in_prev_node with ⟨drop, ih⟩
+        exists ⟨drop.val + 1, by simp⟩
+      | inr term_not_in_prev_node =>
         exists ⟨0, by simp⟩
-        simp [Option.is_some_and]
-        rw [← node_is_at_path]
-        simp
-        have triggers_exist := ct.triggers_exist tail
-        rw [eq] at triggers_exist
-        simp [Option.is_none_or] at triggers_exist
-        cases triggers_exist with
-        | inr no_trg_ex =>
-          unfold not_exists_trigger_list at no_trg_ex
-          have : ct.tree.get (head::tail) = none := by
-            apply ct.tree.each_successor_none_of_children_empty
-            exact no_trg_ex.right
-          rw [this] at node_is_at_path
-          simp at node_is_at_path
-        | inl trg_ex =>
-          unfold exists_trigger_list at trg_ex
-          cases trg_ex with | intro trg' htrg' =>
-            have head_lt_tail_children_length : head < (ct.tree.children tail).length := by
-              apply Decidable.byContradiction
-              intro contra
-              have : none = (ct.tree.children tail)[head]? := by
-                simp at contra
-                apply Eq.symm
-                apply List.getElem?_eq_none
-                exact contra
-              rw [FiniteDegreeTree.getElem_children_eq_getElem_lifted_children] at this
-              rw [PossiblyInfiniteTree.getElem_children_eq_get] at this
-              unfold FiniteDegreeTree.get at node_is_at_path
-              rw [← node_is_at_path] at this
-              contradiction
-            have head_lt_aux_1 : head < trg'.val.mapped_head.length := by rw [← htrg'.right] at head_lt_tail_children_length; simp [List.length_enum_with_lt] at head_lt_tail_children_length; exact head_lt_tail_children_length
-            have head_lt_aux_2 : head < trg'.val.rule.head.length := by rw [← htrg'.right] at head_lt_tail_children_length; simp [List.length_enum_with_lt] at head_lt_tail_children_length; rw [← PreTrigger.length_mapped_head]; exact head_lt_tail_children_length
+        rw [List.drop_zero, eq]
+        rw [Option.is_some_and]
+        rw [Option.is_some_and_iff]
 
-            rw [← ct.tree.getElem_children_eq_get tail ⟨head, head_lt_tail_children_length⟩] at node_is_at_path
-            injection node_is_at_path with node_is_at_path
-
-            have : ∃ f, f ∈ trg'.val.mapped_head[head] ∧ (trg.val.apply_to_var_or_const result_index (VarOrConst.var var)) ∈ f.terms := by
-              cases exis_f with | intro f hf =>
-                exists f
+        let origin := node.origin.get (ct.origin_isSome path i eq)
+        exists origin
+        constructor
+        . simp [origin]
+        . rcases term_in_node with ⟨f, f_mem, t_mem⟩
+          rw [ct.origin_trg_result_yields_next_node_fact _ _ _ eq] at f_mem
+          cases f_mem with
+          | inl f_mem => apply False.elim; apply term_not_in_prev_node; exists f
+          | inr f_mem =>
+            rw [List.mem_toSet] at f_mem
+            unfold ChaseNode.origin_result at f_mem
+            rw [← PreTrigger.apply_subs_for_mapped_head_eq] at f_mem
+            unfold GroundSubstitution.apply_function_free_conj at f_mem
+            rw [List.mem_map] at f_mem
+            rcases f_mem with ⟨a, a_mem, f_mem⟩
+            rw [← f_mem] at t_mem
+            unfold GroundSubstitution.apply_function_free_atom at t_mem
+            rw [List.mem_map] at t_mem
+            rcases t_mem with ⟨voc, voc_mem, t_mem⟩
+            cases voc with
+            | const c => simp [GroundSubstitution.apply_var_or_const, PreTrigger.functional_term_for_var, GroundTerm.func, GroundTerm.const] at t_mem
+            | var v2 =>
+              have v2_front : ¬ v2 ∈ origin.fst.val.rule.frontier := by
+                intro contra
+                rw [PreTrigger.apply_subs_for_var_or_const_eq, PreTrigger.apply_to_var_or_const_frontier_var _ _ _ contra] at t_mem
+                apply term_not_in_prev_node
+                rcases origin.fst.val.rule.frontier_occurs_in_body _ contra with ⟨b, b_mem, v2_mem⟩
+                exists origin.fst.val.subs.apply_function_free_atom b
                 constructor
-                . have f_in_next_step := hf.left
-                  rw [node_is_at_path] at f_in_next_step
-                  simp [← htrg'.right] at f_in_next_step
-                  cases f_in_next_step with
-                  | inr f_in_result =>
-                    rw [List.enum_with_lt_getElem_snd_eq_getElem, List.mem_toSet] at f_in_result
-                    assumption
-                  | inl f_in_j =>
-                    apply False.elim
-                    apply f_not_in_j
-                    exists f
-                    constructor
-                    exact f_in_j
-                    exact hf.right
-                . exact hf.right
+                . have active := ct.origin_trg_is_active path i node eq
+                  apply active.left
+                  rw [List.mem_toSet]
+                  unfold PreTrigger.mapped_body
+                  unfold GroundSubstitution.apply_function_free_conj
+                  apply List.mem_map_of_mem
+                  exact b_mem
+                . rw [← t_mem]
+                  unfold GroundSubstitution.apply_function_free_atom
+                  rw [List.mem_map]
+                  exists VarOrConst.var v2
+              rw [PreTrigger.apply_subs_for_var_or_const_eq, PreTrigger.apply_to_var_or_const_non_frontier_var _ _ _ v2_front] at t_mem
 
-            have : ∃ var2, ¬ var2 ∈ trg'.val.rule.frontier ∧ (trg.val.apply_to_var_or_const result_index (VarOrConst.var var)) = (trg'.val.apply_to_var_or_const head (VarOrConst.var var2)) := by
-              cases this with | intro f hf =>
-                have ⟨f_in_res, apply_var_in_f_terms⟩ := hf
+              have := RTrigger.funcTermForExisVarInMultipleTriggersMeansTheyAreTheSame
+                trg
+                origin.fst
+                ⟨trg_idx.val, by rw [← PreTrigger.length_mapped_head]; exact trg_idx.isLt⟩
+                ⟨origin.snd.val, by rw [← PreTrigger.length_mapped_head]; exact origin.snd.isLt⟩
+                v
+                v2
+                v_front
+                v2_front
+              apply this
+              rw [PreTrigger.apply_to_var_or_const_non_frontier_var _ _ _ v_front]
+              rw [PreTrigger.apply_to_var_or_const_non_frontier_var _ _ _ v2_front]
+              exact Eq.symm t_mem
 
-                let term_for_f := trg'.val.var_or_const_for_result_term ⟨head, head_lt_aux_1⟩ f_in_res apply_var_in_f_terms
-                have h_term_for_f := trg'.val.apply_on_var_or_const_for_result_term_is_term ⟨head, head_lt_aux_1⟩ f_in_res apply_var_in_f_terms
+  theorem funcTermForExisVarInChaseMeansTriggerResultOccurs (ct : ChaseTree obs kb) (path : List Nat) {node : ChaseNode obs kb.rules} (eq : ct.tree.get path = some node)
+      (trg : RTrigger obs kb.rules) (trg_idx : Fin trg.val.mapped_head.length) {v : sig.V} (v_front : ¬ v ∈ trg.val.rule.frontier)
+      (term_in_node : ∃ (f : Fact sig), f ∈ node.fact ∧ (trg.val.functional_term_for_var trg_idx.val v) ∈ f.terms) :
+      trg.val.mapped_head[trg_idx.val].toSet ⊆ node.fact.val := by
+    rcases ct.funcTermForExisVarInChaseMeansTriggerIsUsed path eq trg trg_idx v_front term_in_node with ⟨drop, h⟩
+    rw [Option.is_some_and_iff] at h
+    rcases h with ⟨prev_node, prev_node_eq, h⟩
+    rw [Option.is_some_and_iff] at h
+    rcases h with ⟨origin, origin_eq, h⟩
+    simp only [PreTrigger.result_eq_of_equiv _ _ h.left, h.right]
+    have := prev_node.fact_contains_origin_result
+    rw [origin_eq, Option.is_none_or] at this
+    apply Set.subset_trans this
+    have := ct.stepIsSubsetOfAllFollowing (path.drop drop.val) prev_node prev_node_eq (path.take drop.val)
+    rw [List.take_append_drop, eq, Option.is_none_or] at this
+    exact this
 
-                cases eq : term_for_f with
-                | const c =>
-                  apply False.elim
-                  have contra := h_term_for_f
-                  unfold term_for_f at eq
-                  rw [eq, PreTrigger.apply_to_var_or_const_for_const] at contra
-                  rw [trg.val.apply_to_var_or_const_non_frontier_var result_index _ var_not_in_frontier] at contra
-                  simp [PreTrigger.functional_term_for_var, GroundTerm.const, GroundTerm.func] at contra
-                | var v =>
-                  exists v
-                  unfold term_for_f at eq
-                  rw [eq] at h_term_for_f
-                  constructor
-                  . intro contra
-                    apply f_not_in_j
-                    rcases trg'.val.rule.frontier_occurs_in_body v contra with ⟨body_atom, contra'⟩
-                    exists (trg'.val.subs.apply_function_free_atom body_atom)
-                    constructor
-                    . have trg'_loaded := htrg'.left.left
-                      apply trg'_loaded
-                      rw [List.mem_toSet]
-                      unfold PreTrigger.mapped_body
-                      unfold GroundSubstitution.apply_function_free_conj
-                      apply List.mem_map_of_mem
-                      exact contra'.left
-                    . conv at h_term_for_f => right; unfold PreTrigger.apply_to_var_or_const; unfold PreTrigger.skolemize_var_or_const; rw [Function.comp_apply]
-                      rw [← h_term_for_f]
-                      rw [trg'.val.apply_to_var_or_const_frontier_var head v contra]
-                      unfold GroundSubstitution.apply_function_free_atom
-                      rw [List.mem_map]
-                      exists VarOrConst.var v
-                      simp [GroundSubstitution.apply_var_or_const, contra']
-                  . rw [h_term_for_f]
-
-            have : trg.equiv trg' ∧ result_index.val = head := by
-              cases this with | intro var2 hvar2 =>
-                apply RTrigger.funcTermForExisVarInMultipleTriggersMeansTheyAreTheSame trg trg' ⟨result_index.val, by rw [← PreTrigger.length_mapped_head]; exact result_index.isLt⟩ ⟨head, head_lt_aux_2⟩
-                apply var_not_in_frontier
-                apply hvar2.left
-                apply hvar2.right
-
-            simp [← htrg'.right] at node_is_at_path
-            rw [node_is_at_path]
-            simp
-            rw [List.enum_with_lt_getElem_fst_eq_index head_lt_aux_1]
-            exact this
-
-theorem funcTermForExisVarInChaseTreeMeansTriggerResultOccurs (ct : ChaseTree obs kb) (trg : RTrigger obs kb.rules) (result_index : Fin trg.val.mapped_head.length) (var : sig.V) (node : ChaseNode obs kb.rules) (node_path : List Nat) : (some node = ct.tree.get node_path) ∧ (¬ var ∈ trg.val.rule.frontier) ∧ (∃ (f : Fact sig), f ∈ node.fact ∧ (trg.val.apply_to_var_or_const result_index (VarOrConst.var var)) ∈ f.terms) -> trg.val.mapped_head[result_index.val].toSet ⊆ node.fact := by
-  intro h
-  have node_is_at_path := h.left
-  cases funcTermForExisVarInChaseTreeMeansTriggerIsUsed ct trg result_index var node node_path h with | intro drop_number h =>
-    cases eq : ct.tree.get (node_path.drop drop_number) with
-    | none => rw [eq] at h; simp [Option.is_some_and] at h
-    | some prev_node =>
-      rw [eq] at h; simp [Option.is_some_and] at h
-      have : trg.val.mapped_head[result_index.val].toSet ⊆ prev_node.fact := by
-        cases eq : prev_node.origin with
-        | none => simp [eq] at h
-        | some origin =>
-          have fact_contains_origin_result := prev_node.fact_contains_origin_result
-          simp [eq] at h
-          rw [eq] at fact_contains_origin_result
-          simp [Option.is_none_or] at fact_contains_origin_result
-          simp [h.right]
-          unfold RTrigger.equiv at h
-          simp [PreTrigger.result_eq_of_equiv _ _ h.left]
-          exact fact_contains_origin_result
-
-      apply Set.subset_trans
-      . exact this
-      . have subsetAllFollowing := chaseTreeSetIsSubsetOfAllFollowing ct (node_path.drop drop_number) (node_path.take drop_number)
-        rw [eq] at subsetAllFollowing
-        rw [List.take_append_drop] at subsetAllFollowing
-        rw [← node_is_at_path] at subsetAllFollowing
-        simp [Option.is_none_or] at subsetAllFollowing
-        exact subsetAllFollowing
-
-theorem chaseBranchResultModelsKb (cb : ChaseBranch obs kb) : cb.result.modelsKb kb := by
-  constructor
-  . unfold FactSet.modelsDb
-    unfold ChaseBranch.result
-    intro f h
-    exists 0
-    rw [cb.database_first]
-    simp [Option.is_some_and]
-    exact h
-  . unfold FactSet.modelsRules
-    intro r h
-    unfold FactSet.modelsRule
-    simp
-    intro subs subs_loaded
-    apply Classical.byContradiction
-    intro subs_not_obsolete
-    let trg : Trigger obs := ⟨r, subs⟩
-    have trg_loaded : trg.loaded cb.result := by apply subs_loaded
-    have trg_not_obsolete : ¬ obs.cond trg cb.result := by
-      intro contra
-      have obs_impl_sat := obs.cond_implies_trg_is_satisfied contra
-      apply subs_not_obsolete
-      rcases obs_impl_sat with ⟨i, s', obs_impl_sat⟩
-      exists i
-      exists s'
-
-    cases (trgActiveForChaseResultMeansActiveAtSomeIndex cb trg ⟨trg_loaded, trg_not_obsolete⟩) with | intro i active_i =>
-      have not_active_eventually := cb.fairness ⟨trg, by apply h⟩
-      cases not_active_eventually with | intro j not_active =>
-        have not_active_j := not_active.left
-        simp [Trigger.active] at not_active_j
-        unfold Option.is_some_and at not_active_j
-        split at not_active_j
-        . contradiction
-        case h_2 heq =>
-          have obsolete_j := not_active_j (by
-            simp [PreTrigger.loaded]
-            unfold Option.is_some_and at active_i
-            cases eq : cb.branch.infinite_list i with
-            | none => rw [eq] at active_i; simp at active_i
-            | some step_i =>
-              rw [eq] at active_i; simp at active_i
-              apply Set.subset_trans
-              . apply active_i.left
-              . cases Decidable.em (i ≤ j) with
-                | inl j_ge_i =>
-                  cases Nat.le.dest j_ge_i with | intro m hm =>
-                    have step_i_subs_following := chaseBranchSetIsSubsetOfAllFollowing cb i m
-                    rw [eq] at step_i_subs_following
-                    simp at step_i_subs_following
-                    rw [hm, heq] at step_i_subs_following
-                    simp [Option.is_none_or] at step_i_subs_following
-                    exact step_i_subs_following
-                | inr h =>
-                  have h : j < i := Nat.lt_of_not_le h
-                  have contra := not_active.right i h
-                  rw [eq] at contra
-                  simp [Option.is_none_or] at contra
-                  contradiction
-          )
-          apply trg_not_obsolete
-          apply obs.monotone
-          have step_j_subs_result := chaseBranchSetIsSubsetOfResult cb j
-          rw [heq] at step_j_subs_result
-          simp [Option.is_none_or] at step_j_subs_result
-          exact step_j_subs_result
-          exact obsolete_j
-
-theorem chaseTreeResultModelsKb (ct : ChaseTree obs kb) : ∀ fs, fs ∈ ct.result -> fs.modelsKb kb := by
-  intro fs is_result
-  unfold Set.element at is_result
-  unfold ChaseTree.result at is_result
-  cases is_result with | intro branch h =>
-    rw [← h.right]
-    apply chaseBranchResultModelsKb
+end ChaseTree
 
